Typing respects equivalence of expressions, statements, and contexts.
(We above forced us to allow annotations of differing type in function contexts
(sigma) for typing expressions.)

ott/coq/AilTyping.v
@@ -53,7 +53,7 @@ Definition type_of_constant P ic : option integerType :=
         None
   end.
 
-Definition type_of_rvalue_aux {B} (type_of_expression : expression B -> option typeCategory) e :=
+Definition type_of_rvalue_aux {A} (type_of_expression : expression A -> option typeCategory) e :=
   match type_of_expression e with
   | Some (RValueType   t) => Some (pointer_conversion t)
   | Some (LValueType _ t) => lvalue_conversion t
@@ -69,7 +69,7 @@ Definition well_typed_assignment t1 t2 null2 :=
   | _            , _             => arithmetic t1 && arithmetic t2
   end.
 
-Definition assignable_aux {B} (type_of_rvalue : expression B -> option ctype) :=
+Definition assignable_aux {A} (type_of_rvalue : expression A -> option ctype) :=
   fun t1 e2 =>
     match type_of_rvalue e2 with
     | Some t2 => well_typed_assignment t1 t2 (null_pointer_constant e2)
@@ -89,42 +89,6 @@ Definition well_typed_binary_arithmetic t1 aop t2 : bool :=
   | Xor  => integer    t1 && integer    t2
   | Bor  => integer    t1 && integer    t2
   end.
-
-Definition pointer_to_complete_object t : bool :=
-  match t with
-  | Pointer _ t => complete t
-  | _           => false
-  end.
-
-Definition pointers_to_compatible_complete_objects t1 t2 : bool :=
-  match t1, t2 with
-  | Pointer _ t1, Pointer _ t2 => complete t1 && complete t2 && compatible t1 t2
-  | _           , _            => false
-  end.  
-
-Definition pointers_to_compatible_objects t1 t2 : bool :=
-  match t1, t2 with
-  | Pointer _ t1, Pointer _ t2 => object t1 && object t2 && compatible t1 t2
-  | _           , _            => false
-  end.  
-
-Definition pointer_to_object t : bool :=
-  match t with
-  | Pointer _ t => object t
-  | _           => false
-  end.
-
-Definition pointer_to_void t : bool :=
-  match t with
-  | Pointer _ Void => true
-  | _              => false
-  end.
-
-Definition pointers_to_compatible_types t1 t2 : bool :=
-  match t1, t2 with
-  | Pointer _ t1, Pointer _ t2 => compatible t1 t2
-  | _           , _            => false
-  end.  
 
 Definition well_typed_equality t1 t2 is_null1 is_null2 : bool :=
      pointer t1 && is_null2
@@ -178,16 +142,16 @@ Definition well_typed_conditional P t1 t2 t3 null2 null3 : option typeCategory :
   else
     None.
 
-Definition well_typed_arguments_aux {B : Set} (assignable : ctype -> expression B -> bool) :=
-  fix well_typed_arguments (es : list (expression B)) (ps : list (qualifiers * ctype)) : bool :=
+Definition well_typed_arguments_aux {A : Set} (assignable : ctype -> expression A -> bool) :=
+  fix well_typed_arguments (es : list (expression A)) (ps : list (qualifiers * ctype)) : bool :=
     match es, ps with
     | nil    , nil           => true
     | e :: es, (_, t1) :: ps => assignable (pointer_conversion t1) e && well_typed_arguments es ps 
     | _      , _             => false
     end.
 
-Fixpoint type_of_expression' {A B} P G (S : sigma A B) (e : expression' B) : option typeCategory :=
-  let type_of_rvalue       := type_of_rvalue_aux (type_of_expression P G S) in
+Fixpoint type_of_expression' {A B1 B2} P (S : sigma B1 B2) (G : gamma) (e : expression' A) : option typeCategory :=
+  let type_of_rvalue       := type_of_rvalue_aux (type_of_expression P S G) in
   let assignable           := assignable_aux type_of_rvalue                 in
   let well_typed_arguments := well_typed_arguments_aux assignable           in
   match e with
@@ -202,10 +166,10 @@ Fixpoint type_of_expression' {A B} P G (S : sigma A B) (e : expression' B) : opt
      type_of_rvalue e2 >>= fun t2 =>
      Some (RValueType t2)
   | Unary Address e =>
-      match type_of_expression P G S e with
-      | Some (LValueType q t)             => Some (RValueType (Pointer q t))
-      | Some (RValueType (Function t ps)) => Some (RValueType (Pointer no_qualifiers (Function t ps)))
-      | _                                 => None
+      match type_of_expression P S G e with
+      | Some (LValueType q t)            => Some (RValueType (Pointer q t))
+      | Some (RValueType (Function t p)) => Some (RValueType (Pointer no_qualifiers (Function t p)))
+      | _                                => None
       end
   | Unary Plus e
   | Unary Minus e =>
@@ -233,7 +197,7 @@ Fixpoint type_of_expression' {A B} P G (S : sigma A B) (e : expression' B) : opt
       end
   | Unary PostfixIncr e
   | Unary PostfixDecr e =>
-      match type_of_expression P G S e with
+      match type_of_expression P S G e with
       | Some (LValueType q' t') =>
           lvalue_conversion t' >>= fun t =>
           if modifiable q' t' && (real t' || pointer t')
@@ -249,7 +213,7 @@ Fixpoint type_of_expression' {A B} P G (S : sigma A B) (e : expression' B) : opt
       | _                                  => None
       end
   | Assign e1 e2 =>
-      match type_of_expression P G S e1, type_of_rvalue e2 with
+      match type_of_expression P S G e1, type_of_rvalue e2 with
       | Some (LValueType q1 t1), Some t2 =>
           let t := pointer_conversion t1 in
           if modifiable q1 t1 && assignable t e2
@@ -275,17 +239,17 @@ Fixpoint type_of_expression' {A B} P G (S : sigma A B) (e : expression' B) : opt
       if well_typed_binary_arithmetic t1 aop t2
         then option_map RValueType (promotion P t1)
         else None
-  | Binary e1 (Arithmetic (Add  as aop)) e2 =>
+  | Binary e1 (Arithmetic Add) e2 =>
       type_of_rvalue e1 >>= fun t1 => 
       type_of_rvalue e2 >>= fun t2 =>
       if pointer_to_complete_object t1 && integer t2 then
         Some (RValueType t1)
       else if pointer_to_complete_object t2 && integer t1 then
         Some (RValueType t2)
-      else if well_typed_binary_arithmetic t1 aop t2 then
+      else if well_typed_binary_arithmetic t1 Add t2 then
         option_map RValueType (usual_arithmetic P t1 t2)
       else None
-  | Binary e1 (Arithmetic (Sub  as aop)) e2 =>
+  | Binary e1 (Arithmetic Sub) e2 =>
       type_of_rvalue e1 >>= fun t1 =>
       type_of_rvalue e2 >>= fun t2 =>
       if pointers_to_compatible_complete_objects t1 t2 then
@@ -353,7 +317,7 @@ Fixpoint type_of_expression' {A B} P G (S : sigma A B) (e : expression' B) : opt
       well_typed_conditional P t1 t2 t3 (null_pointer_constant e2) (null_pointer_constant e3)
   | CompoundAssign e1 Add e2
   | CompoundAssign e1 Sub e2 =>
-      match type_of_expression P G S e1, type_of_rvalue e2 with
+      match type_of_expression P S G e1, type_of_rvalue e2 with
       | Some (LValueType q t), Some t2 => 
           lvalue_conversion t >>= fun t1 =>
           if modifiable q t && (arithmetic t1 && arithmetic t2 || pointer_to_complete_object t && integer t2)
@@ -362,7 +326,7 @@ Fixpoint type_of_expression' {A B} P G (S : sigma A B) (e : expression' B) : opt
       | _ , _  => None
       end
   | CompoundAssign e1 aop e2 =>
-      match type_of_expression P G S e1, type_of_rvalue e2 with
+      match type_of_expression P S G e1, type_of_rvalue e2 with
       | Some (LValueType q t), Some t2 => 
           lvalue_conversion t >>= fun t1 =>
           if modifiable q t && well_typed_binary_arithmetic t1 aop t2
@@ -371,22 +335,22 @@ Fixpoint type_of_expression' {A B} P G (S : sigma A B) (e : expression' B) : opt
       | _, _  => None
       end
   end
-with type_of_expression {A B} P G (S : sigma A B) (e : expression B) : option typeCategory :=
+with type_of_expression {A B1 B2} P (S : sigma B1 B2) (G : gamma) (e : expression A) : option typeCategory :=
   match e with
-  | AnnotatedExpression _ e => type_of_expression' P G S e
+  | AnnotatedExpression _ e => type_of_expression' P S G e
   end.
 
-Definition type_of_rvalue {A B} P G (S : sigma A B) : expression B -> option ctype := 
-  type_of_rvalue_aux (type_of_expression P G S).
+Definition type_of_rvalue {A B1 B2} P (S : sigma B1 B2) G : expression A -> option ctype := 
+  type_of_rvalue_aux (type_of_expression P S G).
 
-Definition assignable {A B} P G (S : sigma A B) : ctype -> expression B -> bool :=
-  assignable_aux (type_of_rvalue P G S).
+Definition assignable {A B1 B2} P (S : sigma B1 B2) G : ctype -> expression A -> bool :=
+  assignable_aux (type_of_rvalue P S G).
 
-Definition well_typed_arguments {A B} P G (S : sigma A B) : list (expression B) -> list (qualifiers * ctype) -> bool :=
-  well_typed_arguments_aux (assignable P G S).
+Definition well_typed_arguments {A B1 B2} P (S : sigma B1 B2) G : list (expression A) -> list (qualifiers * ctype) -> bool :=
+  well_typed_arguments_aux (assignable P S G).
 
-Definition typeable {A B} P G (S : sigma A B)  e : bool :=
-  match type_of_expression P G S e with
+Definition typeable {A B1 B2} P (S : sigma B1 B2) G (e : expression A) : bool :=
+  match type_of_expression P S G e with
   | Some _ => true
   | None   => false
   end.
@@ -398,74 +362,74 @@ Definition well_formed_binding (b : identifier * (qualifiers * ctype)) :=
 Definition well_formed_bindings bs :=
   all_list well_formed_binding bs && disjoint_bindings eq_identifier bs.
 
-Definition well_typed_block_aux {A B : Set} (well_typed_statement : statement A B -> bool) :=
+Definition well_typed_block_aux {A1 A2 : Set} (well_typed_statement : statement A1 A2 -> bool) :=
   all_list well_typed_statement.
 
-Definition well_typed_definition {A B : Set} P G (S : sigma A B) (d : identifier * expression B) :=
+Definition well_typed_definition {A B1 B2 : Set} P (S : sigma B1 B2) G (d : identifier * expression A) :=
   let '(v, e) := d in
   match lookup G v with
-  | Some (_, t) => assignable P G S t e
+  | Some (_, t) => assignable P S G t e
   | _           => false
   end.
 
-Definition well_typed_definitions {A B : Set} P G (S : sigma A B) :=
-  all_list (well_typed_definition P G S).
+Definition well_typed_definitions {A B1 B2 : Set} P (S : sigma B1 B2) G (ds : list (identifier * expression A)) :=
+  all_list (well_typed_definition P S G) ds.
 
-Fixpoint well_typed_statement' {A B} P G (S : sigma A B) t_return (s : statement' A B) : bool :=
-  let well_typed_block bs := well_typed_block_aux (well_typed_statement P (add_bindings bs G) S t_return) in
+Fixpoint well_typed_statement' {A1 A2 B1 B2 : Set} P (S : sigma B1 B2) (G : gamma) t_return (s : statement' A1 A2) : bool :=
+  let well_typed_block bs := well_typed_block_aux (well_typed_statement P S (add_bindings bs G) t_return) in
   match s with
-  | Label _ s => well_typed_statement P G S t_return s
+  | Label _ s => well_typed_statement P S G t_return s
   | Case ic s => match type_of_constant P ic with
-                 | Some _ => well_typed_statement P G S t_return s 
+                 | Some _ => well_typed_statement P S G t_return s 
                  | None   => false
                  end
-  | Default s => well_typed_statement P G S t_return s
+  | Default s => well_typed_statement P S G t_return s
   | Block bs ss => well_formed_bindings bs && fresh_bindings bs S && well_typed_block bs ss
   | Skip      => true
-  | Expression e => typeable P G S e
-  | If e s1 s2 => match type_of_rvalue P G S e with
-                  | Some t => scalar t && well_typed_statement P G S t_return s1
-                                       && well_typed_statement P G S t_return s2
+  | Expression e => typeable P S G e
+  | If e s1 s2 => match type_of_rvalue P S G e with
+                  | Some t => scalar t && well_typed_statement P S G t_return s1
+                                       && well_typed_statement P S G t_return s2
                   | None   => false
                   end
-  | Switch e s => match type_of_rvalue P G S e with
-                  | Some t => integer t && well_typed_statement P G S t_return s
+  | Switch e s => match type_of_rvalue P S G e with
+                  | Some t => integer t && well_typed_statement P S G t_return s
                   | None   => false
                   end
-  | While e s => match type_of_rvalue P G S e with
-                 | Some t => scalar t && well_typed_statement P G S t_return s
+  | While e s => match type_of_rvalue P S G e with
+                 | Some t => scalar t && well_typed_statement P S G t_return s
                  | None   => false
                  end
-  | Do s e => match type_of_rvalue P G S e with
-              | Some t => scalar t && well_typed_statement P G S t_return s
+  | Do s e => match type_of_rvalue P S G e with
+              | Some t => scalar t && well_typed_statement P S G t_return s
               | None   => false
               end
   | Goto _    => true
   | Continue  => true
   | Break     => true
   | ReturnVoid => eq_ctype t_return Void
-  | Return e   => assignable P G S t_return e
-  | Declaration ds => well_typed_definitions P G S ds
+  | Return e   => assignable P S G t_return e
+  | Declaration ds => well_typed_definitions P S G ds
   end
-with well_typed_statement {A B} P G (S : sigma A B) t_return (s : statement A B) : bool :=
+with well_typed_statement {A1 A2 B1 B2 : Set} P (S : sigma B1 B2) (G : gamma) t_return (s : statement A1 A2) : bool :=
   match s with
-  | AnnotatedStatement _ s => well_typed_statement' P G S t_return s
+  | AnnotatedStatement _ s => well_typed_statement' P S G t_return s
   end.
 
-Definition well_typed_block {A B} P G (S : sigma A B) t_return :=
-  well_typed_block_aux (well_typed_statement P G S t_return).
+Definition well_typed_block {A1 A2 B1 B2 : Set} P (S : sigma B1 B2) G t_return (ss : list (statement A1 A2)) :=
+  well_typed_block_aux (well_typed_statement P S G t_return) ss.
 
-Definition well_typed_function {A B} P (S : sigma A B) p :=
+Definition well_typed_function {A1 A2 B1 B2 : Set} P (S : sigma B1 B2) (p : _ * _ * statement A1 A2) :=
   let '(t_return, bs, s) := p in
   fresh_bindings bs S &&
   well_formed_bindings bs &&
   wf_type (Function t_return (parameters_of_bindings bs)) &&
-  well_typed_statement P (add_bindings bs empty) S t_return s.
+  well_typed_statement P S (add_bindings bs empty) t_return s.
 
-Definition well_typed_sigma {A B} P (S : sigma A B) : bool :=
+Definition well_typed_sigma {A1 A2} P (S : sigma A1 A2) : bool :=
   Context.all eq_identifier (fun _ => well_typed_function P S) S.
 
-Definition well_typed_program {A B} P (p:program A B) : bool :=
+Definition well_typed_program {A1 A2} P (p:program A1 A2) : bool :=
   let (main, S) := p in
   match lookup S main with
   | Some (Basic (Integer (Signed Int)), nil, _) => well_typed_sigma P S
