ott/coq/AilSyntaxAux_proof.v
@@ -4,8 +4,11 @@ Require Import AilTypesAux AilTypesAux_proof.
 Require Import AilSyntax AilSyntax_proof.
 Require Import AilSyntaxAux.
 
+Module D.
 Require AilSyntaxAux_defns.
-Module D := AilSyntaxAux_defns.
+Include AilSyntax_defns.
+Include AilSyntaxAux_defns.
+End D.
 
 Lemma fv_correct {A} v :
   forall x : expression A, boolSpec (fv v x) (D.fv v x).
@@ -35,4 +38,21 @@ Proof.
   | |- unqualified ?q = _ -> _ => case_fun (unqualified_correct q)
   | _ => context_destruct
   end; now my_auto.
+Qed.
+
+Lemma nullPointerConstant_equiv {A1 A2} :
+  forall {e1 : expression A1} {e2 : expression A2},
+    D.equivExpression e1 e2 ->
+    D.nullPointerConstant e1 ->
+    D.nullPointerConstant e2.
+Proof.
+  apply (
+    expression_nrect
+      (fun x => forall (y : expression' A2) (Hequiv : D.equivExpression' x y) (Hnull1 : D.nullPointerConstant' x), D.nullPointerConstant' y)
+      (fun x => forall y (Hequiv : D.equivExpression x y) (Hnull1 : D.nullPointerConstant x), D.nullPointerConstant y)
+      (fun _ => True)
+  ); intros;
+  first [inversion Hequiv; subst | now trivial];
+  inversion Hnull1; subst;
+  constructor; solve [assumption | apply H; assumption].
 Qed.
